ocaml/src/AstsToSExp.mli
@@ -57,6 +57,10 @@ val nnrs_imp_to_sexp : QLang.nnrs_imp -> sexp
 val sexp_to_imp_qcert : sexp -> QLang.imp_qcert
 val imp_qcert_to_sexp : QLang.imp_qcert -> sexp
 
+val sexp_to_imp_json : sexp -> QLang.imp_json
+val imp_json_to_sexp : QLang.imp_json -> sexp
+
+
 val sexp_to_nnrcmr : sexp -> QLang.nnrcmr
 val nnrcmr_to_sexp : QLang.nnrcmr -> sexp
 
