ocaml/src/QcertOut.ml
@@ -39,6 +39,7 @@ let output_query pconf q =
   | QcertCompiler.Q_nnrs_core q -> pretty_query pconf pretty_nnrs_core q
   | QcertCompiler.Q_nnrs_imp q -> pretty_query pconf pretty_nnrs_imp q
   | QcertCompiler.Q_imp_qcert q -> pretty_query pconf pretty_imp_qcert q
+  | QcertCompiler.Q_imp_json q -> pretty_query pconf pretty_imp_json q
   | QcertCompiler.Q_nnrcmr q -> pretty_query pconf pretty_nnrcmr q
   | QcertCompiler.Q_cldmr q -> pretty_query pconf pretty_cldmr q
   | QcertCompiler.Q_dnnrc q -> pretty_query pconf pretty_dnnrc q
