coq/Imp/Lang/ImpJsonEval.v
@@ -1,0 +1,57 @@
+(*
+ * Copyright 2015-2016 IBM Corporation
+ *
+ * Licensed under the Apache License, Version 2.0 (the "License");
+ * you may not use this file except in compliance with the License.
+ * You may obtain a copy of the License at
+ *
+ * http://www.apache.org/licenses/LICENSE-2.0
+ *
+ * Unless required by applicable law or agreed to in writing, software
+ * distributed under the License is distributed on an "AS IS" BASIS,
+ * WITHOUT WARRANTIES OR CONDITIONS OF ANY KIND, either express or implied.
+ * See the License for the specific language governing permissions and
+ * limitations under the License.
+ *)
+
+(** NNRSimp is a variant of the named nested relational calculus
+     (NNRC) that is meant to be more imperative in feel.  It is used
+     as an intermediate language between NNRC and more imperative /
+     statement oriented backends *)
+
+Require Import String.
+Require Import List.
+Require Import Arith.
+Require Import EquivDec.
+Require Import Morphisms.
+Require Import Arith.
+Require Import Max.
+Require Import Bool.
+Require Import Peano_dec.
+Require Import EquivDec.
+Require Import Decidable.
+Require Import Utils.
+Require Import CommonRuntime.
+Require Import Imp.
+Require Import ImpJson.
+
+Section ImpJsonEval.
+
+  Context {fruntime:foreign_runtime}.
+
+  (* Context (h:brand_relation_t). *)
+
+  (* Local Open Scope imp_json. *)
+  Local Open Scope string.
+
+  (** ** Evaluation Semantics *)
+  Section Evaluation.
+
+    Definition imp_json_eval_top (* (σc:bindings) *) (q:imp_json) : option data (* XXX should be: json!!! XXX *) :=
+       None. (* XXX TODO XXX *)
+
+  End Evaluation.
+
+End ImpJsonEval.
+
+(* Arguments imp_stmt_eval_domain_stack {fruntime h s σc σ₁ σ₂}. *)
